src2/MemoryPerms.v
@@ -1,0 +1,841 @@
+(* begin hide *)
+
+From Coq Require Import
+     Classes.Morphisms
+     Relations.Relation_Operators
+     Logic.JMeq
+     Lists.List
+     Arith.PeanoNat
+     Logic.FunctionalExtensionality
+     Lia.
+
+From ExtLib Require Import
+     Structures.Monads
+     Data.Monads.OptionMonad.
+
+From Heapster2 Require Import
+     Utils
+     Permissions
+     PermissionsSpred2
+     Memory
+     SepStep
+     Typing
+     PermType.
+
+From ITree Require Import
+     ITree
+     ITreeFacts
+     Basics.MonadState
+     Basics.MonadProp
+     Events.State
+     Events.Exception
+     Events.Nondeterminism
+     Eq.Eqit
+     Eq.UpToTaus
+     Eq.EqAxiom.
+
+From Paco Require Import
+     paco.
+
+Import MonadNotation.
+Import ListNotations.
+Import ITreeNotations.
+Local Open Scope itree_scope.
+(* end hide *)
+
+Section MemoryPerms.
+  Context {Si Ss : Type}.
+  Context `{Hlens: Lens Si memory}.
+  Context {Spred : Type}.
+  Context {interp_spred : Spred -> Si * Ss -> Prop}.
+  Context (Hinv : forall spred si ss m,
+              interp_spred spred (si, ss) <->
+                interp_spred spred (lput si m, ss)).
+
+
+  Section asdf.
+  Context (spred : Spred).
+  (** memory helpers **)
+
+  (* Lemma allocated_read c1 c2 ptr : *)
+  (*   read c1 ptr = read c2 ptr -> *)
+  (*   allocated c1 ptr -> *)
+  (*   allocated c2 ptr. *)
+  (* Proof. *)
+  (*   destruct ptr as [b o]. *)
+  (*   unfold read, allocated. simpl. intros. *)
+  (*   destruct (m c1 b), (m c2 b); try solve [inversion H; inversion H0]; auto. *)
+  (*   - destruct l0, l1. *)
+  (*     destruct (bytes o), (bytes0 o); try solve [contradiction]. *)
+  (*     + rewrite (Bool.reflect_iff _ _ (Nat.ltb_spec0 _ _)) in H0. *)
+  (*       rewrite H0 in H. *)
+  (*       destruct (o <? size0) eqn:?; auto. *)
+  (*       rewrite <- (Bool.reflect_iff _ _ (Nat.ltb_spec0 _ _)) in Heqb0. auto. *)
+  (*       inversion H. *)
+  (*     + rewrite (Bool.reflect_iff _ _ (Nat.ltb_spec0 _ _)) in H0. *)
+  (*       rewrite H0 in H. *)
+  (*       destruct (o <? size0); inversion H. *)
+  (*   - destruct l0. destruct (bytes o); try solve [contradiction]. *)
+  (*     rewrite (Bool.reflect_iff _ _ (Nat.ltb_spec0 _ _)) in H0. *)
+  (*     rewrite H0 in H. inversion H. *)
+  (* Qed. *)
+
+  (* Lemma allocated_read' c1 c2 ptr : *)
+  (*   read c1 ptr = read c2 ptr -> *)
+  (*   allocated c1 ptr = allocated c2 ptr. *)
+  (* Proof. *)
+  (* Admitted. *)
+
+  (* Definition alloc_invariant (c1 c2 : config) (ptr : addr) : Prop := *)
+  (*   allocated c1 ptr = allocated c2 ptr. *)
+
+  (* Lemma alloc_invariant_read c1 c2 ptr : *)
+  (*   alloc_invariant c1 c2 ptr -> *)
+  (*   read c2 ptr = None -> *)
+  (*   read c1 ptr = None. *)
+  (* Proof. *)
+  (*   destruct ptr as [b o]. *)
+  (*   unfold alloc_invariant. unfold allocated. unfold read. simpl in *. intros. *)
+  (*   destruct (m c1 b), (m c2 b); try solve [inversion H0]; auto. *)
+  (*   - destruct l0, l1. *)
+  (*     destruct (bytes o), (bytes0 o). *)
+  (*     + destruct (o <? size) eqn:?; auto. *)
+  (*       rewrite <- (Bool.reflect_iff _ _ (Nat.ltb_spec0 _ _)) in Heqb0. *)
+  (*       rewrite H in Heqb0. *)
+  (*       rewrite (Bool.reflect_iff _ _ (Nat.ltb_spec0 _ _)) in Heqb0. *)
+  (*       rewrite Heqb0 in H0. inversion H0. *)
+  (*     + destruct (o <? size) eqn:?; auto. *)
+  (*       rewrite <- (Bool.reflect_iff _ _ (Nat.ltb_spec0 _ _)) in Heqb0. *)
+  (*       rewrite H in Heqb0. inversion Heqb0. *)
+  (*     + destruct (o <? size); auto. *)
+  (*     + destruct (o <? size); auto. *)
+  (*   - destruct l0. destruct (bytes o). *)
+  (*     + destruct (o <? size) eqn:?; auto. *)
+  (*       rewrite <- (Bool.reflect_iff _ _ (Nat.ltb_spec0 _ _)) in Heqb0. *)
+  (*       rewrite H in Heqb0. inversion Heqb0. *)
+  (*     + destruct (o <? size); auto. *)
+    (* Qed. *)
+  (* Abort. *)
+
+  (* Lemma write_success_allocation c c' ptr val : *)
+  (*   write c ptr val = Some c' -> *)
+  (*   alloc_invariant c c' ptr. *)
+  (* Proof. *)
+  (*   destruct ptr as [b o]. *)
+  (*   intros. unfold alloc_invariant. unfold allocated. unfold write in H. simpl in *. *)
+  (*   destruct (m c b) eqn:?; try solve [inversion H]. destruct l0. *)
+  (*   destruct (o <? size) eqn:?; try solve [inversion H]. *)
+  (*   destruct (is_some (bytes o)) eqn:?; try solve [inversion H]. *)
+  (*   inversion H; subst; clear H. simpl. repeat rewrite Nat.eqb_refl. *)
+  (*   destruct (bytes o); auto. inversion Heqb1. *)
+  (* Qed. *)
+
+
+  (* Lemma read_write : forall c ptr, *)
+  (*     (exists val, read c ptr = Some val) -> *)
+  (*     bind (read c ptr) (fun val => write c ptr val) = Some c. *)
+  (* Proof. *)
+  (*   intros. destruct H. simpl. rewrite H. unfold read in H. unfold write. *)
+  (*   destruct ptr as (b & o). destruct c. simpl in *. *)
+  (*   destruct (m0 b) eqn:?; try solve [inversion H]. destruct l1. *)
+  (*   destruct (o <? size); try solve [inversion H]. *)
+  (*   apply f_equal. (* not sure why I need apply *) *)
+  (*   f_equal. apply functional_extensionality. intros. destruct (x0 =? b) eqn:?; auto. *)
+  (*   rewrite <- (Bool.reflect_iff _ _ (Nat.eqb_spec _ _)) in Heqb0; subst. *)
+  (*   rewrite Heqo0. f_equal. f_equal. apply functional_extensionality. intros. *)
+  (*   destruct (x0 =? o) eqn:?; auto. *)
+  (*   rewrite <- (Bool.reflect_iff _ _ (Nat.eqb_spec _ _)) in Heqb0. subst. auto. *)
+  (* Qed. *)
+
+  (* Lemma write_write : forall c ptr val, *)
+  (*     bind (write c ptr val) (fun c' => write c' ptr val) = write c ptr val. *)
+  (* Proof. *)
+  (*   simpl. intros. destruct (write c ptr val) eqn:?; auto. unfold write in *. *)
+  (*   destruct (m c (fst ptr)) eqn:?; try solve [inversion Heqo]. *)
+  (*   destruct l0 eqn:?. destruct (snd ptr <? size) eqn:?; inversion Heqo. *)
+  (*   simpl. rewrite Nat.eqb_refl. rewrite Heqb. apply f_equal. f_equal. *)
+  (*   apply functional_extensionality. intros. destruct (x =? fst ptr); auto. *)
+  (*   repeat f_equal. apply functional_extensionality. intros. *)
+  (*   destruct (x0 =? snd ptr); auto. *)
+  (* Qed. *)
+
+  (** * Memory permissions **)
+
+  (** Gives permission to allocate memory, assuming the last allocated block was [n-1] *)
+  Program Definition malloc_perm (n : nat) : (@perm {x : Si * Ss | interp_spred spred x }) :=
+    {|
+    (** always valid *)
+    pre '(x, _) := length (lget x) = n;
+    (** No new blocks are allocated *)
+    rely '(x, _) '(y, _) := length (lget x) = length (lget y) /\
+                            (forall ptr, fst ptr >= n ->
+                                    sizeof (lget x) ptr = sizeof (lget y) ptr /\
+                                    read (lget x) ptr = read (lget y) ptr);
+    (** Existing blocks do not change *)
+    guar '(x, _) '(y, _) :=
+      (forall ptr, fst ptr < n ->
+              read (lget x) ptr = read (lget y) ptr /\
+              sizeof (lget x) ptr = sizeof (lget y) ptr);
+    |}.
+  Next Obligation.
+    constructor.
+    - intros [[] ?]. cbn. split; auto.
+    - intros [[] ?] [[] ?] [[] ?]. cbn. intros [] []. split. etransitivity; eauto.
+      intros. split.
+      + etransitivity. apply H0; auto. apply H2; auto.
+      + etransitivity. apply H0; auto. apply H2; auto.
+  Qed.
+  Next Obligation.
+    constructor; [intros [[] ?] | intros [[] ?] [[] ?] [[] ?] ? ?]; cbn in *; auto.
+    split; (etransitivity; [apply H; auto |]); apply H0; auto.
+  Qed.
+  Next Obligation.
+    cbn in *. destruct H. rewrite <- H. auto.
+  Qed.
+
+  Program Definition block_perm (size : nat) (ptr : addr) : (@perm { x : (Si * Ss) | interp_spred spred x} ) :=
+    {|
+    (** [ptr] points to the first cell of an allocated block of size [size] *)
+    pre '(x, _) :=
+      (* if we swap the order of the equality then the obligation automatically
+      unifies and we lose info... *)
+      Some size = sizeof (lget x) ptr;
+    (** if [ptr] satisfies the precondition, the size of the block does not change *)
+    rely '(x, _) '(y, _) :=
+      sizeof (lget x) ptr = sizeof (lget y) ptr;
+    (** no updates allowed *)
+    guar '(x, _) '(y, _) := x = y;
+    |}.
+  Next Obligation.
+    constructor; [intros [[] ?] | intros [[] ?] [[] ?] [[] ?]]; cbn in *; etransitivity; eauto.
+  Qed.
+  Next Obligation.
+    constructor; [intros [[] ?] | intros [[] ?] [[] ?] [[] ?]]; cbn in *; etransitivity; eauto.
+  Qed.
+  Next Obligation.
+    cbn in *. rewrite <- H. auto.
+  Qed.
+
+  Lemma malloc_block n size ptr :
+    size > 0 ->
+    fst ptr < n ->
+    malloc_perm n ⊥ block_perm size ptr.
+  Proof.
+    intros Hsize Hn.
+    constructor; intros [[] ?] [[] ?] ?; cbn in *; subst; auto.
+    intros. apply H; auto.
+  Qed.
+
+  Program Definition read_perm (ptr : addr) (v : Value) : @perm ({ x : Si * Ss | interp_spred spred x}) :=
+    {|
+    (** [ptr] points to [v] *)
+    pre '(x, _) := read (lget x) ptr = Some v;
+    (** only checks if the memory [ptr] points to in the 2 memories are equal *)
+    rely '(x, _) '(y, _) := read (lget x) ptr = read (lget y) ptr;
+    (** no updates allowed *)
+    guar '(x, _) '(y, _) := x = y;
+    |}.
+  Next Obligation.
+    constructor; [intros [[] ?] | intros [[] ?] [[] ?] [[] ?]]; cbn in *; auto; etransitivity; eauto.
+  Qed.
+  Next Obligation.
+    constructor; [intros [[] ?] | intros [[] ?] [[] ?] [[] ?]]; cbn in *; auto; etransitivity; eauto.
+  Qed.
+  Next Obligation.
+    cbn in *. rewrite <- H. auto.
+  Qed.
+
+  Program Definition write_perm (ptr : addr) (v : Value) : (@perm {x : Si * Ss | interp_spred spred x}) :=
+    {|
+    (* [ptr] points to [v] *)
+    pre '(x, _) := Some v = read (lget x) ptr;
+    (* only checks if the memory [ptr] points to in the 2 configs are equal *)
+    rely '(x, _) '(y, _) := read (lget x) ptr = read (lget y) ptr;
+    (* only the pointer we have write permission to may change *)
+    guar '(x, _) '(y, _) := (forall ptr', ptr <> ptr' -> read (lget x) ptr' = read (lget y) ptr') /\
+                            (forall ptr', sizeof (lget x) ptr' = sizeof (lget y) ptr') /\
+                            length (lget x) = length (lget y);
+    |}.
+  Next Obligation.
+    constructor; [intros [[] ?] | intros [[] ?] [[] ?] [[] ?]]; cbn in *; auto; etransitivity; eauto.
+  Qed.
+  Next Obligation.
+    constructor; [intros [[] ?] | intros [[] ?] [[] ?] [[] ?] ? ?]; cbn in *; auto.
+    split; [| split]; (etransitivity; [apply H; auto |]); apply H0; auto.
+  Qed.
+  Next Obligation.
+    cbn in *. rewrite <- H. auto.
+  Qed.
+
+  Lemma read_lte_write : forall ptr v, read_perm ptr v <= write_perm ptr v.
+  Proof.
+    constructor; cbn in *; intros [[] ?]; cbn in *; subst; auto. intros [[] ?] ?. cbn in *. subst. auto.
+  Qed.
+
+  Lemma malloc_write : forall n ptr v,
+      fst ptr < n ->
+      malloc_perm n ⊥ write_perm ptr v.
+  Proof.
+    intros n ptr v. constructor; intros [[] ?] [[] ?]; simpl in *; intros.
+    - destruct ptr. split; [| intros [] ?; split]; auto; apply H0;
+                      intro Heq; inversion Heq; subst; lia.
+    - apply H0; auto.
+  Qed.
+
+  Lemma write_block : forall b o o' size v,
+      block_perm size (b, o) ⊥ write_perm (b, o') v.
+  Proof.
+    constructor; intros [[] ?] [[] ?] ?; simpl in *; subst; auto.
+    apply H.
+  Qed.
+
+  Lemma write_write_sep ptr ptr' v v' :
+      ptr <> ptr' ->
+      write_perm ptr v ⊥ write_perm ptr' v'.
+  Proof.
+    intros Hdiff. constructor; intros [[] ?] [[] ?] ?; cbn in *; apply H; auto.
+  Qed.
+
+  Program Definition post_malloc_perm n size : (@perm {x : Si * Ss | interp_spred spred x}) :=
+    {|
+    pre '(x, _) :=
+      length (lget x) = n + 1 /\
+      Some size = sizeof (lget x) (n, 0) /\
+      Some (VNum 0) = read (lget x) (n, 0);
+    rely x y :=
+      rely (malloc_perm (n + 1) ** block_perm size (n, 0) ** write_perm (n, 0) (VNum 0)) x y;
+    rely_PO := rely_PO (malloc_perm (n + 1) ** block_perm size (n, 0) ** write_perm (n, 0) (VNum 0));
+    guar x y :=
+      guar (malloc_perm (n + 1) ** block_perm size (n, 0) ** write_perm (n, 0) (VNum 0)) x y;
+    guar_PO := guar_PO (malloc_perm (n + 1) ** block_perm size (n, 0) ** write_perm (n, 0) (VNum 0));
+    |}.
+  Next Obligation.
+    cbn in *. destruct H. destruct H0 as (? & ? & ?). split; [| split].
+    - rewrite <- H. auto.
+    - rewrite <- H2. auto.
+    - rewrite <- H1. auto.
+  Qed.
+
+  (*
+  (* same spred *)
+  Lemma sep_step_malloc n size : sep_step _ _ _ (fun _ H => H)
+                                          (malloc_perm n)
+                                          (post_malloc_perm n size).
+  Proof.
+    apply sep_step_rg.
+    - intros [si ss] [si' ss'] ?. induction H; try solve [etransitivity; eauto].
+      destruct H.
+      2: { destruct x as [[? ?] ?], y as [[? ?] ?].
+           destruct H as (? & ? & ?). split; auto.
+           apply H; intro Heq; inversion Heq; subst; cbn in *; lia.
+      }
+      induction H; try solve [etransitivity; eauto]. destruct H.
+      + destruct x as [[? ?] ?], y as [[? ?] ?]. split; apply H; lia.
+      + destruct x as [[? ?] ?], y as [[? ?] ?]. cbn in *. subst; auto.
+    - intros [[si ss] ?] [[si' ss'] ?] [Hlen Hptr]. simpl in *.
+      split; [split; [split |] |]; auto; intros; apply Hptr; cbn; lia.
+  Qed.
+   *)
+  (* Lemma read_write_separate_neq_ptr : forall ptr ptr' v v', *)
+  (*     read_perm ptr v ⊥ write_perm ptr' v' <-> ptr <> ptr'. *)
+  (* Proof. *)
+  (*   split; repeat intro. *)
+  (*   - destruct H as [? _]. simpl in *. subst. *)
+  (*     specialize (sep_l (config_mem ptr' (Byte 0)) (config_mem ptr' (Byte 1))). *)
+  (*     do 2 rewrite read_config_mem in sep_l. *)
+  (*     assert (Some (Byte 0) = Some (Byte 1) -> False) by inversion 1. *)
+  (*     apply H. clear H. apply sep_l. split; [| split; [| split]]; auto. *)
+  (*     + intros. unfold read, config_mem. simpl. *)
+  (*       destruct ptr', ptr'0. destruct (addr_neq_cases _ _ _ _ H); simpl in *. *)
+  (*       * rewrite (Bool.reflect_iff _ _ (Nat.eqb_spec _ _)) in H0. *)
+  (*         apply Bool.not_true_is_false in H0. rewrite Nat.eqb_sym in H0. *)
+  (*         rewrite H0. auto. *)
+  (*       * destruct (n1 =? n); auto. destruct (n2 <? n0 + 1); auto. *)
+  (*         rewrite (Bool.reflect_iff _ _ (Nat.eqb_spec _ _)) in H0. *)
+  (*         apply Bool.not_true_is_false in H0. rewrite Nat.eqb_sym in H0. *)
+  (*         rewrite H0. auto. *)
+  (*     + unfold alloc_invariant, allocated, config_mem. simpl. *)
+  (*       repeat rewrite Nat.eqb_refl. auto. *)
+  (*   - constructor; intros; simpl in *; subst; auto. *)
+  (*     destruct H0. auto. *)
+  (* Qed. *)
+
+  (* Lemma write_write_separate_neq_ptr : forall ptr ptr' v v', *)
+  (*     write_perm ptr v ⊥ write_perm ptr' v' <-> ptr <> ptr'. *)
+  (* Proof. *)
+  (*   split; intros. *)
+  (*   - symmetry in H. eapply separate_antimonotone in H. symmetry in H. *)
+  (*     eapply read_write_separate_neq_ptr. apply H. apply read_lte_write. *)
+  (*   - constructor; intros; simpl in *; destruct H0; auto. *)
+  (* Qed. *)
+
+  (* Lemma read_separate : forall ptr ptr' v v', read_perm ptr v ⊥ read_perm ptr' v'. *)
+  (* Proof. *)
+  (*   constructor; intros; simpl in *; subst; reflexivity. *)
+  (* Qed. *)
+  End asdf.
+
+
+  Lemma foo spred spred' Hspred n :
+    restrict (Si * Ss) (interp_spred spred) (interp_spred spred') Hspred (malloc_perm spred' n) ≡≡ malloc_perm spred n.
+  Proof.
+    split; intros.
+    - constructor; intros.
+      + destruct x. auto.
+      + destruct x, y. destruct x, x0. cbn in *. auto.
+      + destruct x, y. destruct x, x0. cbn in *. auto.
+    - constructor; intros.
+      + destruct x. auto.
+      + destruct x, y. destruct x, x0. cbn in *. auto.
+      + destruct x, y. destruct x, x0. cbn in *. auto.
+  Qed.
+
+  (** * Memory mermission sets *)
+  Definition malloc_Perms : Perms2 :=
+    meet_Perms2 (fun Q => exists (n : nat) spred,
+                     Q = singleton_Perms2 (interp_spred spred) (malloc_perm spred n)).
+
+  Definition read_Perms (ptr : addr) (P : Value -> Perms2) : Perms2 :=
+    meet_Perms2 (fun Q => exists (y : Value) spred,
+                     Q = sep_conj_Perms2
+                           (singleton_Perms2 _ (read_perm spred ptr y))
+                           (P y)).
+
+  Definition write_Perms (ptr : addr) (P : Value -> Perms2) : Perms2 :=
+    meet_Perms2 (fun Q => exists (y : Value) spred,
+                     Q = sep_conj_Perms2
+                           (singleton_Perms2 _ (write_perm spred ptr y))
+                           (P y)).
+
+  Definition block_Perms (ptr : addr) (n : nat) : Perms2 :=
+    meet_Perms2 (fun Q => exists spred,
+                     Q = singleton_Perms2 _ (block_perm spred n ptr)).
+
+  (** * Memory operations *)
+  Definition load (v : Value) : itree (sceE Si) Value :=
+    s <- trigger (Modify id);;
+    match v with
+    | VNum _ => throw tt
+    | VPtr p => match read (lget s) p with
+               | None => throw tt
+               | Some b => Ret b
+               end
+    end.
+
+  Definition store (ptr : Value) (v : Value) : itree (sceE Si) Si :=
+    match ptr with
+    | VNum _ => throw tt
+    | VPtr ptr => s <- trigger (Modify (fun s => match write (lget s) ptr v with
+                                            | None => s
+                                            | Some c => (lput s c)
+                                            end)) ;;
+                 match write (lget s) ptr v with
+                 | None => throw tt
+                 | Some c => Ret (lput s c)
+               end
+    end.
+
+  Definition malloc (size : nat) : itree (sceE Si) Value :=
+    s <- trigger (Modify id);; (* do a read first to use length without subtraction *)
+    trigger (Modify (fun s =>
+                       (lput s ((lget s) ++
+                                         [Some (LBlock size
+                                                       (fun o => if o <? size
+                                                              then Some (VNum 0)
+                                                              else None))]))));;
+    Ret (VPtr (length (lget s), 0)).
+
+  Definition free (ptr : Value) : itree (sceE Si) unit :=
+    match ptr with
+    | VNum _ => throw tt
+    | VPtr ptr =>
+      if snd ptr =? 0
+      then
+        s <- trigger (Modify id);;
+        match nth_error (lget s) (fst ptr) with
+        | Some (Some (LBlock size bytes)) =>
+          trigger (Modify (fun s =>
+                             (lput s (replace_list_index
+                                        (lget s)
+                                        (fst ptr)
+                                        (Some (LBlock size (fun o => if o <? size then None else bytes o)))))));;
+          Ret tt
+        | _ => throw tt
+        end
+      else throw tt
+    end.
+
+  (* Example no_error_load s : no_errors (lput s (mem_at (0, 0) (VNum 1))) *)
+  (*                                     (load (VPtr (0, 0))). *)
+  (* Proof. *)
+  (*   pstep. unfold load. rewritebisim @bind_trigger. constructor. *)
+  (*   left. pstep. rewrite lGetPut. constructor. *)
+  (* Qed. *)
+  (* Example no_error_store s : no_errors (lput s (mem_at (0, 0) (VNum 1))) *)
+  (*                                      (store (VPtr (0, 0)) (VNum 2)). *)
+  (* Proof. *)
+  (*   pstep. unfold store. rewritebisim @bind_trigger. constructor. *)
+  (*   left. pstep. rewrite lGetPut. constructor. *)
+  (* Qed. *)
+
+  (* diff spreds *)
+  Lemma sep_step_malloc' n size spred1 spred2 Hspred :
+    sep_step _ _ _ Hspred
+             (malloc_perm spred1 n)
+             (post_malloc_perm spred2 n size).
+  Proof.
+    apply sep_step_rg.
+    - intros x y Hx Hy ?. remember (exist _ _ Hx). remember (exist _ _ Hy).
+      revert x y Hx Hy Heqs Heqs0.
+      induction H; intros; subst; auto.
+      2: { destruct y, x. etransitivity; auto. }
+      destruct H.
+      2: { (* destruct x0 as [[? ?] ?], y0 as [[? ?] ?]. *)
+        destruct x0, y0.
+        destruct H as (? & ? & ?). split; auto.
+        apply H; intro Heq; inversion Heq; subst; cbn in *; lia.
+      }
+      remember (exist _ _ Hx). remember (exist _ _ Hy).
+      revert x0 y0 Hx Hy Heqs Heqs0.
+      induction H; intros; subst; auto.
+      2: { destruct y, x. etransitivity; auto. }
+      destruct H.
+      + destruct x0, y0.
+        split; apply H; lia.
+      + destruct x0, y0.
+        cbn in *. subst; auto.
+    - intros [] [] Hx Hy [Hlen Hptr]. simpl in *.
+      split; [split; [split |] |]; auto; intros; apply Hptr; cbn; lia.
+  Qed.
+
+  Lemma typing_malloc l :
+    @typing
+      Si Ss Spred interp_spred _ _
+      malloc_Perms
+      (fun v _ => match v with
+               | VPtr addr => sep_conj_Perms2
+                               (sep_conj_Perms2
+                                  malloc_Perms
+                                  (block_Perms addr (S l)))
+                               (write_Perms addr (fun _ => bottom_Perms2))
+               | _ => top_Perms2
+               end)
+      (malloc (S l))
+      (Ret tt).
+  Proof.
+    intros spred p si ss Hs Hp Hpre. (* cbn in *. Set Printing All. *)
+    pstep. unfold malloc.
+    destruct Hp as (? & (n & spred' & Hspred) & Hp); subst.
+    destruct Hp as (? & Hp).
+    (* read step *)
+    rewritebisim @bind_trigger. econstructor; eauto; try reflexivity.
+    cbn. reflexivity.
+    (* write step *)
+    rewritebisim @bind_trigger. unfold id. econstructor; eauto.
+    { cbn. (* Unshelve. *)
+      apply Hp in Hpre. apply Hp. simpl in *. rewrite lGetPut.
+      intros ptr Hn. split.
+      - unfold read, allocated. simpl. subst. rewrite nth_error_app_early; auto.
+      - unfold sizeof. simpl. subst. rewrite nth_error_app_early; auto.
+    }
+    (* return *)
+    { repeat intro. apply sep_step_malloc'. red in Hp.
+      symmetry. eapply separate_antimonotone.
+      - symmetry in H. apply H.
+      - rewrite foo in Hp. apply Hp.
+    }
+    { econstructor; eauto.
+      - cbn. repeat rewrite lGetPut. apply Hp in Hpre. simpl in Hpre.
+        split; [| split].
+        + rewrite last_length. lia.
+        + unfold sizeof. simpl.
+          rewrite nth_error_app_last; auto.
+        + unfold read, allocated. simpl. rewrite nth_error_app_last; auto.
+      - simpl. apply Hp in Hpre. cbn in Hpre. rewrite Hpre.
+        eexists. exists (write_perm spred (n, 0) (VNum 0)).
+        split; [| split].
+        + do 2 eexists. split; [| split]; try reflexivity.
+          * eexists. split.
+            -- exists (n + 1). eexists. reflexivity.
+            -- cbn. eexists. red. reflexivity.
+          * eexists. split.
+            -- eexists. reflexivity.
+            -- cbn. eexists. red. reflexivity.
+        + eexists. split.
+          * exists (VNum 0). eexists. reflexivity.
+          * do 2 eexists. split; [| split]; cbn; auto.
+            -- cbn. eexists. red. reflexivity.
+            -- rewrite sep_conj_perm_bottom. rewrite restrict_same. reflexivity.
+        + do 2 rewrite restrict_same. constructor; auto.
+          { intros [[] ?] (? & ? & ?). cbn in *. split; split; auto.
+            - split; [| apply malloc_block; simpl; lia].
+              apply H0.
+            - symmetry. apply separate_sep_conj_perm; symmetry.
+              + apply malloc_write. simpl. lia.
+              + apply write_block.
+              + apply malloc_block; simpl; lia.
+          }
+    }
+    Unshelve. all: try apply Hinv; auto.
+  Qed.
+
+  (*
+  Lemma typing_free ptr (Q : Value -> Perms2) :
+    @typing
+      Si Ss Spred interp_spred _ _
+      (sep_conj_Perms2 (write_Perms ptr Q) (block_Perms ptr 1))
+      (fun _ _ => bottom_Perms2)
+      (free (VPtr ptr))
+      (Ret tt).
+  Proof.
+    intros p si ss Hp Hpre. pstep. unfold free.
+    destruct Hp as (pwrite' & pblock & (? & (v & ?) & Hpwrite) & Hpblock & Hlte); subst.
+    destruct Hpwrite as (pwrite & pv & Hpwrite & Hpv & Hlte').
+    assert (Hoffset : snd ptr = 0).
+    { apply Hlte in Hpre. destruct Hpre as (_ & Hpre & _).
+      apply Hpblock in Hpre. simpl in Hpre. unfold sizeof in Hpre.
+      rewrite (Bool.reflect_iff _ _ (Nat.eqb_spec _ _)).
+      destruct (snd ptr =? 0); inversion Hpre; auto.
+    }
+    rewrite Hoffset. simpl.
+    (* read step *)
+    rewritebisim @bind_trigger. econstructor; auto; try reflexivity.
+    pose proof Hpre as Hpre'. apply Hlte in Hpre'.
+    destruct Hpre' as (Hprewrite & Hpreblock & Hsep).
+    apply Hpblock in Hpreblock. simpl in Hpreblock.
+    unfold sizeof in Hpreblock. rewrite Hoffset in Hpreblock. simpl in Hpreblock.
+    destruct (nth_error (lget si) (fst ptr)) eqn:?; try solve [inversion Hpreblock].
+    destruct o; try solve [inversion Hpreblock].
+    destruct l. inversion Hpreblock; clear Hpreblock; subst.
+    (* write step *)
+    rewritebisim @bind_trigger. unfold id. econstructor; auto.
+    - apply Hlte. constructor 1. left.
+      apply Hlte'. constructor 1. left.
+      apply Hpwrite. simpl.
+      split; [| split]; rewrite lGetPut; simpl; auto.
+      + intros. unfold read. unfold allocated. simpl.
+        destruct ptr as [b o]; destruct ptr' as [b' o'].
+        apply addr_neq_cases in H. simpl.
+        admit. (* break up the <> into cases, then use nth_error_replace_list_index_eq/neq *)
+      + admit.
+      + assert (fst ptr < length (lget si)).
+        { apply nth_error_Some. intro. rewrite H in Heqo. inversion Heqo. }
+        apply replace_list_index_length; auto.
+    - apply sep_step_lte'. apply bottom_perm_is_bottom.
+    - constructor; simpl; auto.
+  Admitted.
+
+  (* Lemma typing_load {R} ptr (Q : Value -> Perms) (r : R) : *)
+  (*   typing *)
+  (*     (read_Perms ptr Q) *)
+  (*     (fun x _ => (read_Perms ptr (eq_p x)) * Q x) *)
+  (*     (load (VPtr ptr)) *)
+  (*     (Ret r). *)
+  (* Proof. *)
+  (*   repeat intro. pstep. unfold load. rewritebisim @bind_trigger. *)
+  (*   econstructor; eauto; try reflexivity. *)
+  (*   destruct H as (? & (? & ?) & ?); subst. *)
+  (*   destruct H1 as (? & ? & ? & ? & ?). simpl in *. *)
+  (*   assert (read (lget c1) ptr = Some x0). *)
+  (*   { apply H2 in H0. destruct H0 as (? & _). apply H in H0. auto. } *)
+  (*   rewrite H3. constructor; eauto. *)
+  (*   simpl. exists x, x1. split; [| split]; eauto. eexists. split; eauto. *)
+  (*   simpl. exists x, bottom_perm. split; [| split]; eauto. *)
+  (*   rewrite sep_conj_perm_bottom. reflexivity. *)
+  (* Qed. *)
+
+  Lemma typing_store {R} ptr val' (P Q : Value -> Perms) (r : R) :
+    typing
+      (write_Perms ptr P * Q val')
+      (fun _ _ => write_Perms ptr Q)
+      (store (VPtr ptr) val')
+      (Ret r).
+  Proof.
+    intros p'' c1 c2 H Hpre. pstep. unfold store. rewritebisim @bind_trigger.
+    destruct H as (p' & q & Hwrite & Hq & Hlte). destruct Hwrite as (? & (v & ?) & Hwrite); subst.
+    destruct Hwrite as (pw & p & Hwritelte & Hp & Hlte'). simpl in *.
+    assert (exists val, read (lget c1) ptr = Some val).
+    {
+      apply Hlte in Hpre. destruct Hpre as (Hpre & _).
+      apply Hlte' in Hpre. destruct Hpre as (Hpre & _).
+      apply Hwritelte in Hpre. eexists. symmetry. apply Hpre.
+    }
+    destruct H as (val & Hread). eapply (read_success_write _ _ _ val') in Hread.
+    destruct Hread as (c' & Hwrite).
+    assert (Hguar : guar p' (c1, c2) ((lput c1 c'), c2)).
+    {
+      apply Hlte'. constructor 1. left. apply Hwritelte. simpl.
+      rewrite lGetPut.
+      split; [| split].
+      + eapply write_success_read_neq; eauto.
+      + eapply write_success_sizeof; eauto.
+      + rewrite lGetPut. eapply write_success_length; eauto.
+    }
+    econstructor; eauto.
+    3: {
+      rewrite Hwrite. constructor; eauto.
+      2: { simpl. eexists. split. exists val'. reflexivity.
+           simpl. eexists. exists q. split; [reflexivity | split]; eauto. reflexivity. }
+      split; [| split].
+      - symmetry. eapply write_success_read_eq; rewrite lGetPut; eauto.
+      - apply Hlte in Hpre. respects. 2: apply Hpre; eauto.
+        apply Hpre. auto.
+      - apply Hlte in Hpre. destruct Hpre as (_ & _ & Hsep). symmetry in Hsep.
+        eapply separate_antimonotone in Hsep; eauto. apply separate_sep_conj_perm_l in Hsep.
+        eapply separate_antimonotone in Hsep; eauto. symmetry. constructor; apply Hsep.
+    }
+    - rewrite Hwrite. apply Hlte. constructor 1. left. auto.
+    - eapply sep_step_lte; eauto. apply sep_step_sep_conj_l.
+      { apply Hlte in Hpre. apply Hpre. }
+      eapply sep_step_lte; eauto. eapply sep_step_lte. apply lte_l_sep_conj_perm.
+      eapply sep_step_lte; eauto.
+      intros ? []. constructor; auto.
+  Qed.
+*)
+
+  (* Lemma typing_store' {R} ptr val' (P : Value -> Perms) (r : R): *)
+  (*   typing *)
+  (*     (write_Perms ptr P) *)
+  (*     (fun _ _ => write_Perms ptr (eq_p val')) *)
+  (*     (store (VPtr ptr) val') *)
+  (*     (Ret r). *)
+  (* Proof. *)
+  (*   assert (bottom_Perms ≡ @eq_p Si Ss _ val' val'). *)
+  (*   { split; repeat intro; simpl; auto. } *)
+  (*   rewrite <- sep_conj_Perms_bottom_identity. rewrite sep_conj_Perms_commut. *)
+  (*   rewrite H. apply typing_store. *)
+  (* Qed. *)
+
+  Definition offset (v : Value) (o : nat) : Value :=
+    match v with
+    | VNum n => VNum (n + o)
+    | VPtr (blk, n) => VPtr (blk, n + o)
+    end.
+
+  Variant RW: Type := R | W.
+
+  Definition ptr_Perms {A} (rw : RW) (p : Value) (a : A) T : @Perms2 (Si * Ss) :=
+    match p with
+    | VNum _ => top_Perms2
+    | VPtr p =>
+        meet_Perms2 (fun P => exists v spred,
+                         P = (singleton_Perms2 _ (match rw with
+                                                  | R => read_perm spred p v
+                                                  | W => write_perm spred p v
+                                                  end)) *2
+                               (v :: T ▷ a))
+    end.
+
+  Definition ptr {A} '(rw, o, T) : VPermType A :=
+    {|
+      ptApp := fun x a => ptr_Perms rw (offset x o) a T;
+    |}.
+
+  Fixpoint arr_perm {A} rw o l T : VPermType (Vector.t A l) :=
+    match l with
+    | 0 => trueP
+    | S l' =>
+        {| ptApp := fun xi xss =>
+                      xi :: ptr (rw, o, T) ▷ Vector.hd xss *2
+                      xi :: arr_perm rw (S o) l' T ▷ Vector.tl xss
+        |}
+    end.
+  Notation "'arr' ( rw , o , l , T )":=(arr_perm rw o l T).
+
+  Definition blockPT l : VPermType unit :=
+    {| ptApp := fun a _ => match a with
+                        | VPtr ptr =>
+                            meet_Perms2 (fun Q => exists spred,
+                                             Q = singleton_Perms2 _ (block_perm spred l ptr))
+                        | _ => top_Perms2
+                        end |}.
+
+  Lemma reach_perm_proper {A} r (T : VPermType A) rw o :
+    Proper (lte_PermType ==> lte_PermType)
+           (fun U : VPermType (list A) => PermType.or (eqp r) (T ⋆ (ptr (rw, o, U)))).
+  Proof.
+    intros T1 T2 Hlte v l spred p Hp. simpl.
+    destruct l as [| ?]; simpl in *; auto.
+    destruct Hp as (pt & pptr & Hpt & Hpptr & Hlte').
+    exists pt, pptr. split; [| split]; auto.
+    clear Hpt. unfold ptr_Perms in *.
+    destruct (offset v o) as [? | l]; auto.
+    destruct Hpptr as (? & (v' & spred' & ?) & Hpptr); subst.
+    destruct Hpptr as (? & ? & ? & ? & ?).
+    eexists. split; eauto. do 2 eexists. split; [| split]; eauto. apply Hlte. auto.
+  Qed.
+
+  Program Definition reach_perm {A}
+          (r : Value) (rw : RW) (o : nat)
+          (T : VPermType A)
+    : VPermType (list A) :=
+    @mu _ _ _ (mu_list A) _ (fixed_point_list _)
+        (fun U => PermType.or (eqp r) (T ⋆ (ptr (rw, o, U))))
+        (reach_perm_proper _ _ _ _).
+
+  Program Definition list_perm rw A (T : VPermType A) : VPermType (list A) :=
+    @mu _ _ _ (mu_list A) _ (fixed_point_list _) (fun U => PermType.or (eqp (VNum 0)) (ptr (rw, 0, T) ⋆ ptr (rw, 1, U))) _.
+  Next Obligation.
+    repeat intro. cbn. induction b; cbn in *; auto.
+    destruct H0 as (? & ? & ? & ? & ?). exists x0, x1. split; auto. split; auto.
+    clear H0. unfold ptr_Perms in *. destruct (offset a 1); auto.
+    destruct H1. destruct H0. destruct H0 as (? & ? & ?); subst.
+    destruct H1 as (? & ? & ? & ? & ?).
+    eexists. split; eauto. do 2 eexists. split; eauto. split; eauto. apply H. auto.
+  Qed.
+
+  Definition list_reach_perm {A} r rw (T : VPermType A) : VPermType (list A) :=
+    reach_perm r rw 1 (ptr (rw, 0, T)).
+
+  Lemma reach_refl {A} x rw o (T : VPermType A) :
+    x :: trueP ▷ tt ⊨2 x :: reach_perm x rw o T ▷ nil.
+  Proof.
+    repeat intro. apply mu_fixed_point. reflexivity.
+  Qed.
+
+  Lemma reach_trans {A} x y z rw o (T : VPermType A) xs ys :
+    x :: reach_perm y rw o T ▷ xs *2 y :: reach_perm z rw o T ▷ ys ⊨2
+    x :: reach_perm z rw o T ▷ (xs ++ ys).
+  Proof.
+    revert x.
+    induction xs.
+    - intros x spred p (p1 & p2 & Hp1 & Hp2 & Hlte).
+      destruct Hp1 as (? & (U & HU & ?) & Hp1); subst.
+      apply HU in Hp1. simpl in Hp1. subst. eapply Perms2_upwards_closed; eauto.
+      red. rewrite restrict_same.
+      etransitivity; eauto. apply lte_r_sep_conj_perm.
+    - intros x spred p (px' & py & Hpx' & Hpy & Hlte).
+      eapply mu_fixed_point in Hpx'.
+      destruct Hpx' as (pa & px & Hpa & Hpx & Hlte').
+      (* x must be a pointer *)
+      destruct x; try contradiction. destruct a0 as [b o'].
+      destruct Hpx as (? & (v & spred' & ?) & Hpx); subst.
+      destruct Hpx as (px'' & pv & Hpx'' & Hpv & Hlte'').
+
+      apply mu_fixed_point. cbn.
+      exists pa. exists (px'' ** (pv ** py)). split; [apply Hpa | split].
+      2: { repeat rewrite <- sep_conj_perm_assoc.
+           etransitivity; eauto.
+           eapply sep_conj_perm_monotone; intuition.
+           repeat rewrite sep_conj_perm_assoc.
+           etransitivity; eauto.
+           eapply sep_conj_perm_monotone; intuition.
+      }
+      eexists; split; [do 2 eexists; reflexivity |].
+      apply sep_conj_Perms2_perm; [apply Hpx'' |].
+      simpl. exists (v :: reach_perm z rw o T ▷ (xs ++ ys)). split.
+      2: { apply IHxs. apply sep_conj_Perms2_perm; auto. }
+      eexists; split; eauto.
+      repeat intro. eapply mu_fixed_point in H; auto.
+      Unshelve. all: auto; apply reach_perm_proper.
+  Qed.
+
+End MemoryPerms.
+
+Notation "'arr' ( rw , o , l , T )" := (arr_perm rw o l T) (at level 40).
+
+
+Inductive LifetimeClauses :=
+| Empty : LifetimeClauses
+| Clause : nat -> nat -> LifetimeClauses -> LifetimeClauses
+.
