src2/PermType.v
@@ -1,0 +1,251 @@
+(* begin hide *)
+From Coq Require Import
+     Classes.Morphisms
+     Relations.Relation_Operators
+     Logic.JMeq
+     Lists.List
+     Arith.PeanoNat
+     Logic.FunctionalExtensionality.
+
+From ExtLib Require Import
+     Structures.Monads
+     Data.Monads.OptionMonad.
+
+From Heapster2 Require Import
+     Utils
+     Permissions
+     PermissionsSpred2
+     Memory
+     SepStep
+     Typing.
+
+From ITree Require Import
+     ITree
+     ITreeFacts
+     Basics.MonadState
+     Basics.MonadProp
+     Events.State
+     Events.Exception
+     Events.Nondeterminism
+     Eq.Eqit
+     Eq.UpToTaus
+     Eq.EqAxiom.
+
+From Paco Require Import
+     paco.
+
+Import MonadNotation.
+(* end hide *)
+
+Section permType.
+  Context {Si Ss : Type}.
+
+  (** * Permission types *)
+
+  Record PermType (A B : Type) : Type :=
+    { ptApp : A -> B -> @Perms2 (Si * Ss) }.
+  Definition VPermType A := PermType Value A.
+  Notation "xi :: T ▷ xs" := (ptApp _ _ T xi xs) (at level 35).
+
+  Definition withPerms {Ai As} (T : PermType Ai As) (P : @Perms2 (Si * Ss)) : PermType Ai As:=
+    {| ptApp:= fun ai abs => (ai :: T ▷ abs) *2 P |}.
+  Notation "T ∅ P" := (withPerms T P) (at level 40).
+
+  Definition plusPT {A1 A2 B1 B2}
+             (T1 : PermType A1 B1) (T2 : PermType A2 B2) : PermType (A1 + A2) (B1 + B2) :=
+    {| ptApp := fun eithA eithB =>
+                  match (eithA, eithB) with
+                  | (inl a1, inl b1) => a1 :: T1 ▷ b1
+                  | (inr a2, inr b2) => a2 :: T2 ▷ b2
+                  | _ => top_Perms2
+                  end |}.
+  Notation "T1 ⊕ T2" := (plusPT T1 T2) (at level 50).
+
+  Definition timesPT {A1 A2 B1 B2}
+             (T1 : PermType A1 B1) (T2 : PermType A2 B2) : PermType (A1 * A2) (B1 * B2) :=
+    {| ptApp := fun a12 b12 => fst a12 :: T1 ▷ fst b12 *2 snd a12 :: T2 ▷ snd b12 |}.
+  Notation "T1 ⊗ T2" := (timesPT T1 T2) (at level 40).
+
+  Definition starPT {Ai As Bs} (T1 : PermType Ai As) (T2 : PermType Ai Bs)
+    : PermType Ai (As * Bs) :=
+    {| ptApp := fun ai abs => (ai :: T1 ▷ fst abs) *2 (ai :: T2 ▷ snd abs) |}.
+  Notation "T1 ⋆ T2" := (starPT T1 T2) (at level 40).
+
+  Definition existsPT {Ai As} {Bs : As -> Type}
+             (F : forall a, PermType Ai (Bs a)) : PermType Ai (sigT Bs) :=
+    {| ptApp := fun ai abs => ai :: F (projT1 abs) ▷ (projT2 abs) |}.
+  Notation "'ex' ( x 'oftype' A ) T" := (existsPT (As:=A) (fun x => T)) (at level 70).
+
+  Definition or {Ai As Bs} (T1 : PermType Ai As)
+             (T2:PermType Ai Bs) : PermType Ai (As + Bs) :=
+    {| ptApp := fun ai abs =>
+                  sum_rect _ (ptApp _ _ T1 ai) (ptApp _ _ T2 ai) abs |}.
+
+  Definition trueP {A B} : PermType A B :=
+    {| ptApp := fun _ _ => bottom_Perms2 |}.
+  Definition falseP {A B} : PermType A B :=
+    {| ptApp := fun _ _ => top_Perms2 |}.
+
+  Program Definition eqp {A} (a : A): PermType A unit :=
+    {| ptApp := fun a' _ => {| in_Perms2 _ _ := a = a' |} |}.
+
+  (** * Operations used in typing rules *)
+
+  Definition vsingle {A} (a:A) : Vector.t A 1 :=
+    Vector.cons _ a _ (Vector.nil _).
+
+  Definition ifz {A} n (x y:A) : A :=
+    if Nat.eqb n 0 then x else y.
+
+  Definition getNum {S} v : itree (sceE S) nat :=
+    match v with VNum n => Ret n | VPtr _ => throw tt end.
+
+  Definition isNull {S} v: itree (sceE S) bool :=
+    match v with
+    | VNum n => if Nat.eqb n 0 then Ret true else throw tt
+    | VPtr _ => Ret false
+    end.
+
+  Definition isNat := ex (n oftype nat) (eqp (VNum n)).
+
+  (** * Recursive and reachability permissions *)
+
+  (** The ordering on permission types is just the lifting of that on Perms *)
+  Definition lte_PermType {A B} (T1 T2 : PermType A B): Prop :=
+    forall a b, lte_Perms2 (ptApp _ _ T1 a b) (ptApp _ _ T2 a b).
+
+  (** Equals on PermType is just the symmetric closure of the ordering *)
+  Definition eq_PermType {A B} (T1 T2 : PermType A B): Prop :=
+    lte_PermType T1 T2 /\ lte_PermType T2 T1.
+
+  Global Instance PreOrder_lte_PermType A B : PreOrder (@lte_PermType A B).
+  Proof.
+    constructor; intro; intros; intros a b.
+    - reflexivity.
+    - etransitivity; [ apply H | apply H0 ].
+  Qed.
+
+  Global Instance Equivalence_eq_PermType A B : Equivalence (@eq_PermType A B).
+  Proof.
+    constructor; intro; intros.
+    - split; reflexivity.
+    - destruct H; split; assumption.
+    - destruct H; destruct H0; split; etransitivity; eassumption.
+  Qed.
+
+  Global Instance Proper_eq_PermType_ptApp A B :
+    Proper (eq_PermType ==> eq ==> eq ==> eq_Perms2) (ptApp A B).
+  Proof.
+    intros T1 T2 eT a1 a2 ea b1 b2 eb. rewrite ea; rewrite eb.
+    destruct eT. split; [ apply H | apply H0 ].
+  Qed.
+
+  (** The meet on permission types is just the lifitng of that on Perms *)
+  Definition meet_PermType {A B} (Ts : PermType A B -> Prop) : PermType A B :=
+    {| ptApp := fun a b => meet_Perms2 (fun P => exists T, Ts T /\ P = (a :: T ▷ b)) |}.
+
+  (** Meet is a lower bound for PermType *)
+  Lemma lte_meet_PermType {A B} (Ts : PermType A B -> Prop) T:
+    Ts T -> lte_PermType (meet_PermType Ts) T.
+  Proof.
+    intros ts_t a b. simpl. apply lte_meet_Perms2. exists T; split; eauto.
+  Qed.
+
+  (** Meet is the greatest lower bound for PermType *)
+  Lemma meet_PermType_max {A B} (Ts : PermType A B -> Prop) T:
+    (forall T', Ts T' -> lte_PermType T T') ->
+    lte_PermType T (meet_PermType Ts).
+  Proof.
+    intros lte_T_Ts a b. apply meet_Perms2_max. intros P [ T' [ Ts_T' P_eq ]].
+    rewrite P_eq. apply (lte_T_Ts T' Ts_T' a b).
+  Qed.
+
+  (** The least fixed-point permission type is defined via the standard
+  Knaster-Tarski construction as the meet of all F-closed permission types *)
+  Definition fixPT {A B} (F : PermType A B -> PermType A B)
+             {prp : Proper (lte_PermType ==> lte_PermType) F} : PermType A B :=
+    meet_PermType (fun T => lte_PermType (F T) T).
+
+  (** First we prove that fixPT is itself F-closed *)
+  Lemma fixPT_F_closed {A B} (F : PermType A B -> PermType A B)
+        {prp : Proper (lte_PermType ==> lte_PermType) F} :
+    lte_PermType (F (fixPT F)) (fixPT F).
+  Proof.
+    intros a b. apply meet_PermType_max. intros T' lte_FT'.
+    transitivity (F T'); [ | assumption ]. apply prp.
+    apply lte_meet_PermType. assumption.
+  Qed.
+
+  (** Then we prove that fixPT is a fixed-point *)
+  Lemma fixPT_fixed_point {A B} (F : PermType A B -> PermType A B)
+        {prp : Proper (lte_PermType ==> lte_PermType) F} :
+    eq_PermType (fixPT F) (F (fixPT F)).
+  Proof.
+    split; [ | apply fixPT_F_closed ].
+    apply lte_meet_PermType. apply prp. apply fixPT_F_closed.
+  Qed.
+
+  Class FixedPoint (G : Type -> Type) X : Type :=
+    { foldFP : G X -> X;
+      unfoldFP : X -> G X;
+      foldUnfold : forall gx, unfoldFP (foldFP gx) = gx;
+      unfoldFold : forall x, foldFP (unfoldFP x) = x; }.
+  Definition unmaprPT {A B C} (f:B -> C) (T:PermType A C) : PermType A B :=
+    {| ptApp := fun a b => a :: T ▷ (f b) |}.
+
+  Program Definition mu {A G X} `{FixedPoint G X}
+             (F : PermType A X -> PermType A (G X))
+             {prp : Proper (lte_PermType ==> lte_PermType) F}
+    : PermType A X :=
+    @fixPT A X (fun T => unmaprPT unfoldFP (F T)) _.
+  Next Obligation.
+    intros T1 T2 leqT a x. simpl. apply prp. assumption.
+  Defined.
+
+  Lemma mu_fixed_point {A G X} `{FixedPoint G X}
+        (F : PermType A X -> PermType A (G X))
+        {prp : Proper (lte_PermType ==> lte_PermType) F} :
+    eq_PermType (mu F) (unmaprPT unfoldFP (F (mu F))).
+  Proof.
+    apply (fixPT_fixed_point (fun T : PermType A X => unmaprPT unfoldFP (F T))).
+  Qed.
+
+  Lemma mu_fixed_point' {A G X} `{FixedPoint G X}
+        (F : PermType A X -> PermType A (G X))
+        {prp : Proper (lte_PermType ==> lte_PermType) F} :
+    lte_PermType (unmaprPT unfoldFP (F (mu F))) (mu F).
+  Proof.
+    apply (fixPT_fixed_point (fun T : PermType A X => unmaprPT unfoldFP (F T))).
+  Qed.
+
+  Definition mu_list A := fun R => sum unit (A * R).
+  Global Program Instance fixed_point_list A : FixedPoint (mu_list A) (list A)
+    :=
+    {
+      foldFP := fun s => match s with
+                      | inl _ => @nil A
+                      | inr (h, t) => (cons h t)
+                      end;
+      unfoldFP := fun l => match l with
+                        | nil => inl tt
+                        | cons h t => inr _ (h, t)
+                        end;
+    }.
+  Next Obligation.
+    destruct gx.
+    - destruct u. auto.
+    - destruct p. auto.
+  Defined.
+  Next Obligation.
+    destruct x; auto.
+  Defined.
+
+End permType.
+
+Notation "P ⊢ ti ⤳ ts ::: U" := (typing P (@ptApp _ _ _ _ U) ti ts) (at level 60).
+Notation "xi :: T ▷ xs" := (@ptApp _ _ _ _ T xi xs) (at level 35).
+Notation "T1 ⊕ T2" := (@plusPT _ _ _ _ _ _ T1 T2) (at level 50).
+Notation "T1 ⊗ T2" := (@timesPT _ _ _ _ _ _ T1 T2) (at level 40).
+Notation "T1 ⋆ T2" := (@starPT _ _ _ _ _ T1 T2) (at level 40).
+Notation "'ex' ( x 'oftype' A ) T" := (@existsPT _ _ _ A _ (fun x => T)) (at level 70).
+Notation "T ∅ P" := (@withPerms _ _ _ _ T P) (at level 40).
